version.v
@@ -10,6 +10,7 @@ Unset Printing Implicit Defensive.
 
 Notation versionUR A := (authR (max_prefix_listUR A)).
 Notation versionG Σ A := (inG Σ (versionUR A)).
+Notation versionΣ A := (GFunctor (versionUR A)).
 
 Section Version.
 
@@ -21,17 +22,26 @@ Context `{!versionG Σ A}.
 
 Implicit Types (x y z : A) (xs ys zs : list A).
 
-Definition version_auth γ dq n x : iProp := ∃ xs,
+Definition version_auth_def γ dq n x : iProp := ∃ xs,
   own γ (●{dq} to_max_prefix_list (xs ++ [x]) ⋅
          ◯     to_max_prefix_list (xs ++ [x])) ∗
   ⌜n = length xs⌝.
+Definition version_auth_aux : seal version_auth_def. by eexists. Qed.
+Definition version_auth := unseal version_auth_aux.
+Lemma version_auth_eq : version_auth = version_auth_def.
+Proof. exact: seal_eq. Qed.
 
-Definition version_frag γ n t : iProp := ∃ ts,
+Definition version_frag_def γ n t : iProp := ∃ ts,
   own γ (◯ to_max_prefix_list (ts ++ [t])) ∗
   ⌜n = length ts⌝.
+Definition version_frag_aux : seal version_frag_def. by eexists. Qed.
+Definition version_frag := unseal version_frag_aux.
+Lemma version_frag_eq : version_frag = version_frag_def.
+Proof. exact: seal_eq. Qed.
 
 Lemma version_alloc x : ⊢ |==> ∃ γ, version_auth γ (DfracOwn 1) 0 x.
 Proof.
+rewrite version_auth_eq.
 iMod (own_alloc (● to_max_prefix_list [x] ⋅
                  ◯ to_max_prefix_list [x])) as "[%γ own]".
   rewrite auth_both_valid; split; eauto.
@@ -39,45 +49,117 @@ iMod (own_alloc (● to_max_prefix_list [x] ⋅
 iModIntro. iExists γ, []. rewrite /=. iFrame. by eauto.
 Qed.
 
+(* FIXME: What if A is not discrete? *)
+Lemma version_auth_dfrac_op `{OfeDiscrete A} γ dq1 dq2 n x :
+  version_auth γ (dq1 ⋅ dq2) n x ⊣⊢
+  version_auth γ dq1 n x ∗ version_auth γ dq2 n x.
+Proof.
+rewrite version_auth_eq. iSplit.
+- iIntros "(%xs & [[own1 own2] #own'] & %en)".
+  iSplitL "own1".
+  + iExists xs. rewrite own_op. by iFrame; iSplit.
+  + iExists xs. rewrite own_op. by iFrame; iSplit.
+- iIntros "[v1 v2]".
+  iDestruct "v1" as "(%xs1 & [own1 #own1'] & %en1)".
+  iDestruct "v2" as "(%xs2 & [own2 #own2'] & %en2)".
+  iPoseProof (own_valid_2 with "own1 own2") as "%valid".
+  have {}valid := auth_auth_dfrac_op_inv _ _ _ _ valid.
+  have e := to_max_prefix_list_inj _ _ valid.
+  have : take n (xs1 ++ [x]) ≡ take n (xs2 ++ [x]) by rewrite e.
+  rewrite !take_app_alt // => <- {xs2 en2 valid e}.
+  iExists xs1. rewrite own_op auth_auth_dfrac_op own_op. iFrame.
+  by iSplit.
+Qed.
+
+Lemma version_auth_discard γ dq n x :
+  version_auth γ dq n x ==∗
+  version_auth γ DfracDiscarded n x.
+Proof.
+rewrite version_auth_eq.
+iIntros "(%xs & [own #own'] & %en)".
+iExists xs. rewrite own_op. do 2!iSplitL => //.
+iApply (own_update with "own").
+apply auth_update_auth_persist.
+Qed.
+
+#[global]
+Instance version_auth_from_sep `{OfeDiscrete A} γ dq1 dq2 n x :
+  FromSep (version_auth γ (dq1 ⋅ dq2) n x)
+          (version_auth γ dq1 n x)
+          (version_auth γ dq2 n x).
+Proof. by rewrite /FromSep version_auth_dfrac_op. Qed.
+
+#[global]
+Instance version_auth_into_sep `{OfeDiscrete A} γ dq1 dq2 n x :
+  IntoSep (version_auth γ (dq1 ⋅ dq2) n x)
+          (version_auth γ dq1 n x)
+          (version_auth γ dq2 n x).
+Proof. by rewrite /IntoSep version_auth_dfrac_op. Qed.
+
+#[global]
+Instance version_auth_timeless γ dq n x `{OfeDiscrete A} :
+  Timeless (version_auth γ dq n x).
+Proof. rewrite version_auth_eq. apply _. Qed.
+
+#[global]
+Instance version_auth_discarded_persistent γ n x :
+  Persistent (version_auth γ DfracDiscarded n x).
+Proof.
+rewrite version_auth_eq /version_auth_def.
+apply: bi.exist_persistent => xs.
+rewrite own_op; apply _.
+Qed.
+
 #[global]
 Instance version_frag_persistent γ n x : Persistent (version_frag γ n x).
-Proof. apply _. Qed.
+Proof. rewrite version_frag_eq. apply _. Qed.
+
+#[global]
+Instance version_frag_timeless γ n x `{OfeDiscrete A} :
+  Timeless (version_frag γ n x).
+Proof. rewrite version_frag_eq. apply _. Qed.
 
 Lemma version_auth_frag γ dq n x : version_auth γ dq n x -∗ version_frag γ n x.
 Proof.
+rewrite version_auth_eq version_frag_eq.
 iDestruct 1 as "(%xs & [own1 #own2] & %nE)".
 iExists xs; eauto.
 Qed.
 
-Lemma version_update γ n x y :
-  version_auth γ (DfracOwn 1) n x ==∗ version_auth γ (DfracOwn 1) (n + 1) y.
+Lemma version_update y γ n x :
+  version_auth γ (DfracOwn 1) n x ==∗ version_auth γ (DfracOwn 1) (S n) y.
 Proof.
+rewrite version_auth_eq.
 iDestruct 1 as "(%xs & own & ->)".
 iMod (own_update with "own") as "own".
   eapply auth_update.
   apply (max_prefix_list_local_update _ ((xs ++ [x]) ++ [y])).
   by exists [y].
-iModIntro. rewrite plus_comm /=.
-iExists (xs ++ [x]). rewrite own_op app_length. iFrame.
-iPureIntro. simpl. lia.
+iModIntro.
+iExists (xs ++ [x]). rewrite own_op app_length plus_comm. iFrame.
+by iPureIntro.
 Qed.
 
 (* FIXME: What if A is not discrete? *)
-Lemma version_auth_agree `{OfeDiscrete A} γ dq1 dq2 n x y :
+Lemma version_auth_agree `{OfeDiscrete A} γ dq1 dq2 n m x y :
   version_auth γ dq1 n x -∗
-  version_auth γ dq2 n y -∗
-  x ≡ y.
+  version_auth γ dq2 m y -∗
+  ⌜n = m ∧ x ≡ y⌝.
 Proof.
+rewrite version_auth_eq.
 iIntros "(%xs & [own_x _] & %e1)".
 iIntros "(%ys & [own_y _] & %e2)".
 iPoseProof (own_valid_2 with "own_x own_y") as "%valid".
 have {}valid := auth_auth_dfrac_op_inv _ _ _ _ valid.
 have e := to_max_prefix_list_inj _ _ valid.
+have elen : length (xs ++ [x]) = length (ys ++ [y]) by rewrite e.
+have enm : n = m by rewrite e1 e2 !app_length /= in elen *; lia.
+iSplit => //.
 have ex : last (xs ++ [x]) = Some x by rewrite last_snoc.
 have ey : last (ys ++ [y]) = Some y by rewrite last_snoc.
 iAssert (Some x ≡ Some y)%I as "e".
   by rewrite -ex -ey e.
-by rewrite option_equivI.
+by rewrite option_equivI; iPoseProof "e" as "%".
 Qed.
 
 (* FIXME: What if A is not discrete? *)
@@ -86,6 +168,7 @@ Lemma version_auth_frag_agree `{OfeDiscrete A} γ dq n x y :
   version_frag γ    n y -∗
   x ≡ y.
 Proof.
+rewrite version_auth_eq version_frag_eq.
 iIntros "(%xs & [own_x _] & %e1)".
 iIntros "(%ys & own_y & %e2)".
 iPoseProof (own_valid_2 with "own_x own_y") as "%valid".
@@ -105,4 +188,27 @@ iAssert (Some x ≡ Some y)%I as "e".
 by rewrite option_equivI.
 Qed.
 
+(* FIXME: What if A is not discrete? *)
+Lemma version_auth_frag_num `{OfeDiscrete A} γ dq n m x y :
+  version_auth γ dq n x -∗
+  version_frag γ    m y -∗
+  ⌜m ≤ n⌝.
+Proof.
+rewrite version_auth_eq version_frag_eq.
+iIntros "(%xs & [own_x _] & %e1)".
+iIntros "(%ys & own_y & %e2)".
+iPoseProof (own_valid_2 with "own_x own_y") as "%valid".
+rewrite auth_both_dfrac_valid_discrete to_max_prefix_list_included in valid.
+case: valid => [] _ [] [zs e] _.
+iPureIntro.
+have : length (ys ++ [y]) ≤ length (xs ++ [x]).
+  rewrite e !app_length; lia.
+rewrite !app_length -e1 -e2 /=; lia.
+Qed.
+
 End Version.
+
+Arguments version_auth {Σ A _}.
+Arguments version_frag {Σ A _}.
+Arguments version_alloc {Σ A _} x.
+Arguments version_update {Σ A _} y.
