pk_dh.v
@@ -139,7 +139,7 @@ iDestruct (dh_seed_elim2 with "priv_nI p_kS") as "[>p_sI >contra]".
 by iDestruct (dh_seed_elim0 with "priv_nR contra") as ">[]".
 Qed.
 
-Lemma wp_pk_dh_init c kI kR dq T E :
+Lemma wp_pk_dh_init c kI kR dq n T E :
   ↑cryptisN ⊆ E →
   ↑N ⊆ E →
   channel c -∗
@@ -147,10 +147,10 @@ Lemma wp_pk_dh_init c kI kR dq T E :
   ctx N -∗
   pterm (TKey Enc kI) -∗
   pterm (TKey Enc kR) -∗
-  {{{ init_confirm kI kR ∗ ●H{dq} T }}}
+  {{{ init_confirm kI kR ∗ ●H{dq|n} T }}}
     pk_dh_init c (TKey Dec kI) (TKey Enc kI) (TKey Enc kR) @ E
   {{{ (okS : option term), RET repr okS;
-      ●H{dq} T ∗
+      ●H{dq|n} T ∗
       if okS is Some kS then
         sterm kS ∗
         □ pk_dh_confirmation Init kI kR kS ∗
@@ -178,17 +178,17 @@ iFrame. do 2!iSplit => //. iModIntro.
 by iApply pk_dh_session_key_elim.
 Qed.
 
-Lemma wp_pk_dh_resp c kR dq T E :
+Lemma wp_pk_dh_resp c kR dq n T E :
   ↑cryptisN ⊆ E →
   ↑N ⊆ E →
   channel c -∗
   cryptis_ctx -∗
   ctx N -∗
   pterm (TKey Enc kR) -∗
-  {{{ resp_confirm kR ∗ ●H{dq} T }}}
+  {{{ resp_confirm kR ∗ ●H{dq|n} T }}}
     pk_dh_resp c (TKey Dec kR) (TKey Enc kR) @ E
   {{{ (res : option (term * term)), RET repr res;
-      ●H{dq} T ∗
+      ●H{dq|n} T ∗
       if res is Some (pkI, kS) then ∃ kI,
         ⌜pkI = TKey Enc kI⌝ ∗
         pterm pkI ∗
