pk_dh_game.v
@@ -55,7 +55,7 @@ Lemma wp_game (mkchan : val) :
   enc_pred_token ⊤ -∗
   key_pred_token (⊤ ∖ ↑nroot.@"keys") -∗
   nown_token session_name ⊤ -∗
-  ●H ∅ -∗
+  ●H{0} ∅ -∗
   WP game mkchan {{ v, ⌜v = NONEV ∨ v = SOMEV #true⌝ }}.
 Proof.
 iIntros "wp_mkchan #ctx enc_tok key_tok nown_tok hon"; rewrite /game; wp_pures.
@@ -88,7 +88,7 @@ wp_pures.
 case: bool_decide_reflect => [ekt|_]; last by wp_pures; iLeft.
 wp_pures; wp_bind (par _ _).
 case: kt epkR' ekt => // -> _.
-rewrite -Qp_half_half -dfrac_op_own. iDestruct "hon" as "[hon1 hon2]".
+rewrite -Qp_quarter_quarter -dfrac_op_own. iDestruct "hon" as "[hon1 hon2]".
 iApply (wp_par (λ v, ∃ a : option term, ⌜v = repr a⌝ ∗ _)%I
                (λ v, ∃ a : option (term * term), ⌜v = repr a⌝ ∗ _)%I
           with "[tokenI hon1] [tokenR hon2]").
@@ -115,7 +115,7 @@ iApply (wp_par (λ v, ∃ a : option term, ⌜v = repr a⌝ ∗ _)%I
 iIntros (v1 v2) "[H1 H2]".
 iDestruct "H1" as (a) "[-> [hon1 H1]]".
 iDestruct "H2" as (b) "[-> [hon2 H2]]".
-iCombine "hon1 hon2" as "hon". rewrite dfrac_op_own Qp_half_half.
+iCombine "hon1 hon2" as "hon". rewrite dfrac_op_own Qp_quarter_quarter.
 iModIntro.
 iMod (compromise_honest with "ctx hon") as "[hon comp]" => //.
 wp_pures.
